Define more of the FOL types by hand.
A pretty good demonstration of how far the nomdatatype package still has to
go.

examples/logic/foltypesScript.sml
@@ -28,15 +28,16 @@ val lp = ``
      n = 0 ∧ (∃s. d = ftmFN s) ∧ (∀i. MEM i uns ⇒ i = 0) ∧ tns = [] ∨
      n = 1 ∧ (∃s. d = ftmRN s) ∧ (∀i. MEM i uns ⇒ i = 0) ∧ tns = [] ∨
      n = 1 ∧ d = ftmF ∧ uns = [] ∧ tns = [] ∨
-     n = 1 ∧ d = ftmIMP ∧ uns = [0;0] ∧ tns = [] ∨
+     n = 1 ∧ d = ftmIMP ∧ uns = [1;1] ∧ tns = [] ∨
      n = 1 ∧ d = ftmALL ∧ uns = [] ∧ tns = [1])
 ``
 
 val {term_ABS_pseudo11, term_REP_11, genind_term_REP, genind_exists,
-     termP, absrep_id, repabs_pseudo_id, term_REP_t, term_ABS_t, newty, ...} =
+     termP, absrep_id, repabs_pseudo_id, term_REP_t, term_ABS_t,
+     newty = term_ty, ...} =
     new_type_step1 tyname 0 {vp=vp, lp = lp}
 
-val VAR_t = mk_var("VAR", ``:string -> ^newty``)
+val VAR_t = mk_var("VAR", ``:string -> ^term_ty``)
 val VAR_def = new_definition(
   "VAR_def",
   ``^VAR_t s = ^term_ABS_t (GVAR s ())``);
@@ -45,7 +46,7 @@ val VAR_termP = prove(
   srw_tac[][genind_rules]);
 val VAR_t = defined_const VAR_def
 
-val FN_t = mk_var("FN", ``:string -> ^newty list -> ^newty``)
+val FN_t = mk_var("FN", ``:string -> ^term_ty list -> ^term_ty``)
 val FN_def = new_definition(
   "FN_def",
   ``^FN_t s args =
@@ -71,24 +72,103 @@ val {tpm_thm = tpm_thm0, term_REP_tpm, t_pmact_t, tpm_t} =
                          term_REP_t = term_REP_t,
                          term_ABS_t = term_ABS_t, absrep_id = absrep_id,
                          repabs_pseudo_id = repabs_pseudo_id,
-                         cons_info = tm_cons_info, newty = newty,
+                         cons_info = tm_cons_info, newty = term_ty,
                          genind_term_REP = genind_term_REP}
 
-val tpm_thm = tpm_thm0
-                  |> SIMP_RULE bool_ss [listpm_MAP, listTheory.MAP_MAP_o,
-                                        combinTheory.o_DEF, SYM term_REP_tpm]
-                  |> REWRITE_RULE [GSYM combinTheory.o_DEF,
-                                   GSYM listTheory.MAP_MAP_o]
-                  |> REWRITE_RULE [FN_def']
+val tpm_thm = save_thm(
+  "tpm_thm",
+  tpm_thm0 |> SIMP_RULE bool_ss [listpm_MAP, listTheory.MAP_MAP_o,
+                                 combinTheory.o_DEF, SYM term_REP_tpm]
+           |> REWRITE_RULE [GSYM combinTheory.o_DEF,
+                            GSYM listTheory.MAP_MAP_o]
+           |> REWRITE_RULE [FN_def']);
 
-(* val {term_ABS_pseudo11 = form_ABS_pseudo11,
-     term_REP_11 = form_REP_11,
-     genind_term_REP = genind_form_REP,
-     genind_exists,
-     termP = formP,
-     absrep_id = form_absrep_id,
-     repabs_pseudo_id = form_repabs_pseudo_id,
-     term_REP_t = form_REP_t, term_ABS_t = form_ABS_t, newty = formty, ...} =
-    new_type_step1 "form" 1 {vp=vp, lp = lp} *)
+val forms_exist = prove(
+  ``∃x. genind ^vp ^lp 1 x``,
+  qexists_tac `GLAM ARB (ftmRN s) [] []` >>
+  match_mp_tac glam >> simp[] >> qexists_tac `[]` >> simp[]);
+
+val {absrep_id, newty = form_ty,
+     repabs_pseudo_id, termP = formP, termP_exists,
+     termP_term_REP = formP_form_REP,
+     term_ABS_t = form_ABS_t, term_ABS_pseudo11 = form_ABS_pseudo11,
+     term_REP_t = form_REP_t, term_REP_11} =
+    newtypeTools.rich_new_type ("form", forms_exist)
+
+val ALL_t = mk_var("ALL", ``:string -> ^form_ty -> ^form_ty``)
+val ALL_def = new_definition(
+  "ALL_def",
+  ``^ALL_t s body =
+    ^form_ABS_t (GLAM s ftmALL [^form_REP_t body] [])``);
+val ALL_formP = prove(
+  mk_comb(formP, ALL_def |> SPEC_ALL |> concl |> rhs |> rand),
+  match_mp_tac glam >> simp[formP_form_REP]);
+val ALL_t = defined_const ALL_def
+
+val REL_t = mk_var("REL", ``:string -> ^term_ty list -> ^form_ty``)
+val REL_def = new_definition(
+  "REL_def",
+  ``^REL_t s args =
+    ^form_ABS_t (GLAM ARB (ftmRN s) [] (MAP ^term_REP_t args))``);
+val REL_formP = prove(
+  ``^formP (GLAM v (ftmRN s) [] (MAP ^term_REP_t args))``,
+  match_mp_tac glam >> simp[genind_term_REP] >>
+  qexists_tac `GENLIST (\n. 0) (LENGTH args)` >>
+  simp[listTheory.MEM_GENLIST,
+       listTheory.LIST_REL_EL_EQN, listTheory.EL_MAP, genind_term_REP])
+val REL_t = defined_const REL_def
+val REL_def' = prove(
+  ``^form_ABS_t (GLAM v (ftmRN s) [] (MAP ^term_REP_t args)) = ^REL_t s args``,
+  srw_tac[][REL_def, GLAM_NIL_EQ, form_ABS_pseudo11, REL_formP]);
+
+val FALSE_t = mk_var("FALSE", ``:^form_ty``)
+val FALSE_def = new_definition(
+  "FALSE_def",
+  ``^FALSE_t = ^form_ABS_t (GLAM ARB ftmF [] [])``);
+val FALSE_formP = prove(
+  ``^formP (GLAM v ftmF [] [])``,
+  match_mp_tac glam >> simp[]);
+val FALSE_t = defined_const FALSE_def
+val FALSE_def' = prove(
+  ``^form_ABS_t (GLAM v ftmF [] []) = ^FALSE_t``,
+  srw_tac[][FALSE_def, GLAM_NIL_EQ, form_ABS_pseudo11, FALSE_formP])
+
+val IMP_t = mk_var("IMP", ``:^form_ty -> ^form_ty -> ^form_ty``)
+val IMP_def = new_definition("IMP_def",
+  ``^IMP_t f1 f2 =
+    ^form_ABS_t (GLAM ARB ftmIMP [] [^form_REP_t f1; ^form_REP_t f2])``);
+val IMP_formP = prove(
+  ``^formP (GLAM v ftmIMP [] [^form_REP_t f1; ^form_REP_t f2])``,
+  match_mp_tac glam >> simp[formP_form_REP]);
+val IMP_t = defined_const IMP_def
+val IMP_def' = prove(
+  ``^form_ABS_t (GLAM v ftmIMP [] [^form_REP_t f1; ^form_REP_t f2]) =
+    ^IMP_t f1 f2``,
+  rw[IMP_def, GLAM_NIL_EQ, form_ABS_pseudo11, IMP_formP]);
+
+val fm_cons_info = [{con_termP = REL_formP, con_def = GSYM REL_def'},
+                    {con_termP = ALL_formP, con_def = ALL_def},
+                    {con_termP = FALSE_formP, con_def = GSYM FALSE_def'},
+                    {con_termP = IMP_formP, con_def = GSYM IMP_def'}]
+val tpm_name_pfx = "f"
+
+val {tpm_thm = fpm_thm0, term_REP_tpm = form_REP_fpm, t_pmact_t = f_pmact_t,
+     tpm_t = fpm_t} =
+    define_permutation { name_pfx = "f", name = "form",
+                         term_REP_t = form_REP_t,
+                         term_ABS_t = form_ABS_t, absrep_id = absrep_id,
+                         repabs_pseudo_id = repabs_pseudo_id,
+                         cons_info = fm_cons_info, newty = form_ty,
+                         genind_term_REP = formP_form_REP}
+
+val fpm_thm = save_thm(
+  "fpm_thm",
+  fpm_thm0 |> SIMP_RULE bool_ss [listpm_MAP, listTheory.MAP_MAP_o,
+                                 combinTheory.o_DEF, SYM term_REP_tpm]
+           |> REWRITE_RULE [GSYM combinTheory.o_DEF,
+                            GSYM listTheory.MAP_MAP_o]
+           |> REWRITE_RULE [REL_def'])
+
+
 
 val _ = export_theory()
